pulse/share/steel/examples/pulse/dice/dpe/DPE.fsti
@@ -1,22 +1,17 @@
 module DPE
-open FStar.Ghost
-open Steel.ST.Util
-open Steel.FractionalPermission
-open Pulse.Steel.Wrapper
-module W = Pulse.Steel.Wrapper
+open Pulse.Lib.Pervasives
 open HACL
 open X509
 open EngineTypes
 open EngineCore
 open L0Types
 open L0Core
-module L = Steel.ST.SpinLock
-module A = Steel.ST.Array
-module R = Steel.ST.Reference
+module L = Pulse.Lib.SpinLock
+module A = Pulse.Lib.Array
+module R = Pulse.Lib.Reference
 module US = FStar.SizeT
 module U8 = FStar.UInt8
 module U32 = FStar.UInt32
-open Array
 open LinearScanHashTable
 open PulseHashTable
 module PHT = PulseHashTable
@@ -33,12 +28,12 @@ type l1_context = { deviceID_priv: A.larray U8.t (US.v v32us);
 
 let l1_context_perm (c:l1_context)
   : vprop
-  = exists_ (fun s -> A.pts_to c.deviceID_priv full_perm s) `star`
-    exists_ (fun s -> A.pts_to c.deviceID_pub full_perm s) `star`
-    exists_ (fun s -> A.pts_to c.aliasKey_priv full_perm s) `star`
-    exists_ (fun s -> A.pts_to c.aliasKey_pub full_perm s) `star`
-    exists_ (fun s -> A.pts_to c.aliasKeyCRT full_perm s) `star`
-    exists_ (fun s -> A.pts_to c.deviceIDCSR full_perm s) `star`
+  = exists_ (fun s -> A.pts_to c.deviceID_priv full_perm s) **
+    exists_ (fun s -> A.pts_to c.deviceID_pub full_perm s) **
+    exists_ (fun s -> A.pts_to c.aliasKey_priv full_perm s) **
+    exists_ (fun s -> A.pts_to c.aliasKey_pub full_perm s) **
+    exists_ (fun s -> A.pts_to c.aliasKeyCRT full_perm s) **
+    exists_ (fun s -> A.pts_to c.deviceIDCSR full_perm s) **
     pure (
       A.is_full_array c.deviceID_priv /\
       A.is_full_array c.deviceID_pub /\
@@ -110,7 +105,7 @@ val prng (_:unit) : nat
 
 val init_l0_ctxt (cdi:A.larray U8.t (US.v dice_digest_len)) (#s:erased (elseq U8.t dice_digest_len))
   : stt locked_context_t
-    (A.pts_to cdi full_perm s `star` pure (A.is_full_array cdi))
+    (A.pts_to cdi full_perm s ** pure (A.is_full_array cdi))
     (fun _ -> A.pts_to cdi full_perm s)
 
 val init_l1_ctxt (deviceIDCSR_len: US.t) (aliasKeyCRT_len: US.t) 
@@ -121,16 +116,16 @@ val init_l1_ctxt (deviceIDCSR_len: US.t) (aliasKeyCRT_len: US.t)
                 (#s5:erased (elseq U8.t deviceIDCSR_len))
                 (#s6:erased (elseq U8.t aliasKeyCRT_len))
   : stt locked_context_t
-     (A.pts_to deviceID_priv full_perm s1 `star` 
-      A.pts_to deviceID_pub full_perm s2 `star`  
-      A.pts_to aliasKey_priv full_perm s3 `star`  
-      A.pts_to aliasKey_pub full_perm s4 `star`  
-      A.pts_to deviceIDCSR full_perm s5 `star` 
+     (A.pts_to deviceID_priv full_perm s1 ** 
+      A.pts_to deviceID_pub full_perm s2 **  
+      A.pts_to aliasKey_priv full_perm s3 **  
+      A.pts_to aliasKey_pub full_perm s4 **  
+      A.pts_to deviceIDCSR full_perm s5 ** 
       A.pts_to aliasKeyCRT full_perm s6) 
      (fun _ -> 
-      A.pts_to deviceID_priv full_perm s1 `star`  
-      A.pts_to deviceID_pub full_perm s2 `star` 
-      A.pts_to aliasKey_priv full_perm s3 `star`  
-      A.pts_to aliasKey_pub full_perm s4 `star`  
-      A.pts_to deviceIDCSR full_perm s5 `star` 
+      A.pts_to deviceID_priv full_perm s1 **  
+      A.pts_to deviceID_pub full_perm s2 ** 
+      A.pts_to aliasKey_priv full_perm s3 **  
+      A.pts_to aliasKey_pub full_perm s4 **  
+      A.pts_to deviceIDCSR full_perm s5 ** 
       A.pts_to aliasKeyCRT full_perm s6)
