pulse/share/steel/examples/pulse/dice/engine/EngineTypes.fst
@@ -1,17 +1,10 @@
 module EngineTypes
-open Pulse.Main
-open Pulse.Steel.Wrapper
-open Steel.ST.Util 
-open Steel.ST.Array
-open Steel.FractionalPermission
-open FStar.Ghost
-module R = Steel.ST.Reference
-module A = Steel.ST.Array
-module T = FStar.Tactics
+open Pulse.Lib.Pervasives
+module R = Pulse.Lib.Reference
+module A = Pulse.Lib.Array
 module US = FStar.SizeT
 module U8 = FStar.UInt8
 open HACL
-open Array
 
 assume
 val uds_is_enabled : vprop
@@ -31,8 +24,8 @@ noeq
 type engine_context = { uds: A.larray U8.t (US.v uds_len); }
 
 let engine_context_perm (c:engine_context) : vprop
-  = A.pts_to c.uds full_perm uds_bytes `star` 
-    uds_is_enabled `star`
+  = A.pts_to c.uds full_perm uds_bytes ** 
+    uds_is_enabled **
     pure (A.is_full_array c.uds)
 
 let mk_engine_context uds : engine_context = {uds}
@@ -64,8 +57,8 @@ let mk_engine_repr  l0_image_header_size l0_image_header l0_image_header_sig
 
 let engine_record_perm (record:engine_record_t) (repr:engine_record_repr) 
   : vprop = 
-  A.pts_to record.l0_image_header full_perm repr.l0_image_header `star`
-  A.pts_to record.l0_image_header_sig full_perm repr.l0_image_header_sig `star`
-  A.pts_to record.l0_binary full_perm repr.l0_binary `star`
-  A.pts_to record.l0_binary_hash full_perm repr.l0_binary_hash `star`
+  A.pts_to record.l0_image_header full_perm repr.l0_image_header **
+  A.pts_to record.l0_image_header_sig full_perm repr.l0_image_header_sig **
+  A.pts_to record.l0_binary full_perm repr.l0_binary **
+  A.pts_to record.l0_binary_hash full_perm repr.l0_binary_hash **
   A.pts_to record.l0_image_auth_pubkey full_perm repr.l0_image_auth_pubkey
