pulse/share/steel/examples/pulse/dice/l0/L0Types.fst
@@ -1,17 +1,5 @@
 module L0Types
-open Pulse.Steel.Wrapper
-open Steel.ST.Util 
-open Steel.ST.Array
-open Steel.FractionalPermission
-open FStar.Ghost
-module R = Steel.ST.Reference
-module A = Steel.ST.Array
-module T = FStar.Tactics
-module US = FStar.SizeT
-module U8 = FStar.UInt8
-module U32 = FStar.UInt32
-open Array
-open HACL
+open Pulse.Lib.Pervasives
 
 let x509_version_t : Type0 = admit()
 
